theories/models/utp_vdm_simple/utp_vdm_sorts.thy
@@ -264,31 +264,89 @@ lemma prjTYPE_vdmval_FuncT [simp]:
 done
 *)
 
-definition binding_fmap ::
-  "'VALUE WF_BINDING \<Rightarrow> 'VALUE ALPHABET \<Rightarrow> ('VALUE VAR, 'VALUE) fmap" where
-"binding_fmap b a = list_fmap (map (\<lambda> x. (x, \<langle>b\<rangle>\<^sub>b x)) (flist a))"
+definition WF_BINDING_MAP :: "('VALUE VAR, 'VALUE) fmap set" where
+"WF_BINDING_MAP = {f. \<forall>x. x \<in>\<^sub>f fdom f \<longrightarrow> the (\<langle>f\<rangle>\<^sub>m x) \<rhd> x}"
 
-lemma "Fmap.fdom (binding_fmap b a) = a"
-  apply (simp add:binding_fmap_def)
-  oops
+definition binding_fmap ::
+  "'VALUE ALPHABET \<Rightarrow> 'VALUE WF_BINDING \<Rightarrow> ('VALUE VAR, 'VALUE) fmap" where
+"binding_fmap a b = list_fmap (map (\<lambda> x. (x, \<langle>b\<rangle>\<^sub>b x)) (flist a))"
+
+lemma binding_fmap_rep_eq: 
+  assumes "x \<in>\<^sub>f a"
+  shows "\<langle>binding_fmap a b\<rangle>\<^sub>m x = Some (\<langle>b\<rangle>\<^sub>b x)"
+proof -
+  obtain xs where fset: "a = fset xs" and lprops: "sorted xs" "distinct xs"
+    by (metis flist_inv flist_props)
+
+  with assms have "x \<in>\<^sub>f fset xs"
+    by simp
+
+  with lprops have "\<langle>binding_fmap (fset xs) b\<rangle>\<^sub>m x = Some (\<langle>b\<rangle>\<^sub>b x)"
+    apply (induct xs)
+    apply (simp add: binding_fmap_def list_fmap.rep_eq)+
+    apply (subgoal_tac "flist (finsert xa (fset xs)) = (xa # flist (fset xs))")
+    apply (simp add: sorted_Cons)
+    apply (metis)
+    apply (metis (lifting) distinct.simps(2) fset_cons fset_inv sorted_Cons)
+  done
+
+  with fset show ?thesis
+    by (simp)
+qed
+
+lemma fdom_binding_map [simp]:
+  "fdom (binding_fmap a b) = a"
+  by (auto simp add:binding_fmap_def)
+
+lemma binding_fmap [closure]:
+  "binding_fmap a b \<in> WF_BINDING_MAP"
+  apply (unfold WF_BINDING_MAP_def)
+  apply (rule CollectI)
+  apply (rule allI)
+  apply (simp add:binding_fmap_rep_eq)
+done
 
 definition fmap_binding ::
   "('VALUE VAR, 'VALUE) fmap \<Rightarrow> 'VALUE WF_BINDING" where
 "fmap_binding f = Abs_WF_BINDING (\<lambda> x. if (x \<in>\<^sub>f Fmap.fdom f) then the (\<langle>f\<rangle>\<^sub>m x) else default (vtype x))"
 
-lemma "fmap_binding (binding_fmap b a) \<cong> b on \<langle>a\<rangle>\<^sub>f"
-  oops
+lemma fmap_binding_rep_eq:
+  "f \<in> WF_BINDING_MAP \<Longrightarrow> 
+   \<langle>fmap_binding f\<rangle>\<^sub>b = (\<lambda> x. if (x \<in>\<^sub>f Fmap.fdom f) then the (\<langle>f\<rangle>\<^sub>m x) else default (vtype x))"
+  apply (subgoal_tac "(\<lambda> x. if (x \<in>\<^sub>f Fmap.fdom f) then the (\<langle>f\<rangle>\<^sub>m x) else default (vtype x)) \<in> WF_BINDING")
+  apply (simp add:fmap_binding_def)
+  apply (unfold WF_BINDING_def)
+  apply (unfold WF_BINDING_MAP_def)
+  apply (rule CollectI)
+  apply (rule allI)
+  apply (case_tac "v \<in>\<^sub>f fdom f")
+  apply (auto intro:typing defined)
+done
 
+lemma binding_fmap_inv:
+  "fmap_binding (binding_fmap a b) \<cong> b on \<langle>a\<rangle>\<^sub>f"
+  by (simp add:binding_equiv_def closure fmap_binding_rep_eq binding_fmap_rep_eq)
 
-(*
-definition predicate_lists :: 
-  "'VALUE WF_PREDICATE \<Rightarrow> 'VALUE ALPHABET \<Rightarrow> ('VALUE list) set" where
-"predicate_lists p a = (\<lambda> b. map \<langle>b\<rangle>\<^sub>b (flist a)) ` destPRED p"
+definition predicate_maps :: 
+  "'VALUE ALPHABET \<Rightarrow>    'VALUE WF_PREDICATE \<Rightarrow> ('VALUE VAR, 'VALUE) fmap set" where
+"predicate_maps a p = binding_fmap a ` destPRED p"
 
-definition lists_predicate :: 
-  "('VALUE list) set \<Rightarrow> 'VALUE ALPHABET \<Rightarrow> 'VALUE WF_PREDICATE" where
-"lists_predicate vs a = mkPRED {b. }"
-*)
+definition maps_predicate :: 
+  "('VALUE VAR, 'VALUE) fmap set \<Rightarrow> 'VALUE WF_PREDICATE" where
+"maps_predicate fs = mkPRED {b. \<exists>f\<in>fs. fmap_binding f \<cong> b on \<langle>fdom f\<rangle>\<^sub>f}"
 
+lemma predicate_maps_inv[simp]:
+  "maps_predicate (predicate_maps (\<alpha> p) (\<pi> p)) = \<pi> p"
+  apply (simp add:maps_predicate_def predicate_maps_def)
+  apply (subgoal_tac "\<And> b f. (fmap_binding (binding_fmap (\<alpha> p) f) \<cong> b on \<langle>\<alpha> p\<rangle>\<^sub>f) = f \<cong> b on \<langle>\<alpha> p\<rangle>\<^sub>f")
+  apply (safe)
+  apply (smt UNIV_I WF_ALPHA_PREDICATE_binding_equiv mem_Collect_eq mkPRED_inverse)
+  apply (simp)
+  apply (rule_tac x="x" in bexI)
+  apply (metis binding_fmap_inv)
+  apply (simp)
+  apply (metis (lifting) binding_equiv_comm binding_equiv_trans binding_fmap_inv)
+  apply (metis (lifting) binding_equiv_trans binding_fmap_inv)
+done
 
 end
